
\subsubsection{Finite Sums}
\begin{equation*} \begin{split}
	\sum_{k=1}^n k   &= \frac{n(n+1)}{2} \\
	\sum_{k=1}^n k^2 &= \frac{n(n+1)(2n+1)}{6} \\
	\sum_{k=0}^n z^k &= \frac{1-z^{n+1}}{1-z} \\
	\sum_{k=0}^n z^k &= \frac{1-z^{n+1}}{1-z}
\end{split} \end{equation*}


\subsubsection{Infinite Sums}
\begin{align*}
	\sum_{n=k}^\infty x^n  &= \frac{x^k}{1-x}    &  0 \le x < 1 \\
	\sum_{n=k}^\infty nx^n &= \frac{kx^k}{1-x} + \frac{x^{k+1}}{(1-x)^2}  &  0 \le x < 1 \\
	\sum_{k=0}^\infty \frac{z^k}{k!} & = e^z  & \\
	\sum_{k=0}^\infty k \frac{z^k}{k!} & = ze^z & \\
	{a \choose k} &= \frac{a!}{k!(a-k)!} & \\
	\sum_{k=0}^\infty  {a \choose k} z^k &= (1+z)^a &
\end{align*}
